@prefix apc: <http://linked.data.gov.au/dataset/apc/> .
@prefix apni: <http://linked.data.gov.au/dataset/apni/> .
@prefix biod: <http://linked.data.gov.au/def/biodiversity/> .
@prefix corveg: <http://linked.data.gov.au/dataset/corveg/> .
@prefix corveg-def: <http://linked.data.gov.au/def/corveg/> .
@prefix cv-corveg: <http://linked.data.gov.au/def/corveg-cv/> .
@prefix data: <http://linked.data.gov.au/def/tern-plot-data/> .
@prefix dct: <http://purl.org/dc/terms/> .
@prefix dist-corveg: <http://linked.data.gov.au/dataset/corveg/disturbance/> .
@prefix dwct: <http://rs.tdwg.org/dwc/terms/> .
@prefix epsg-crs: <http://www.opengis.net/def/crs/epsg/0/> .
@prefix geo: <http://www.w3.org/2003/01/geo/wgs84_pos#> .
@prefix geol-corveg: <http://linked.data.gov.au/dataset/corveg/geology/> .
@prefix location-corveg: <http://linked.data.gov.au/dataset/corveg/location/> .
@prefix locn: <http://www.w3.org/ns/locn#> .
@prefix ogroup-corveg: <http://linked.data.gov.au/def/corveg-ogroup/> .
@prefix op-corveg: <http://linked.data.gov.au/def/corveg-op/> .
@prefix owl: <http://www.w3.org/2002/07/owl#> .
@prefix plot: <http://linked.data.gov.au/def/tern-plot/> .
@prefix prov: <http://www.w3.org/ns/prov#> .
@prefix rdf: <http://www.w3.org/1999/02/22-rdf-syntax-ns#> .
@prefix rdfs: <http://www.w3.org/2000/01/rdf-schema#> .
@prefix rfstruct-corveg: <http://linked.data.gov.au/dataset/corveg/rf-structure/> .
@prefix site-corveg: <http://linked.data.gov.au/dataset/corveg/site/> .
@prefix site-strata-corveg: <http://linked.data.gov.au/dataset/corveg/site-strata/> .
@prefix site-tax-strata-corveg: <http://linked.data.gov.au/dataset/corveg/site-tax-strata/> .
@prefix situation-corveg: <http://linked.data.gov.au/dataset/corveg/situation/> .
@prefix skos: <http://www.w3.org/2004/02/skos/core#> .
@prefix soil-corveg: <http://linked.data.gov.au/dataset/corveg/soil/> .
@prefix soil-text-corveg: <http://registry.it.csiro.au/sandbox/soil-data-ie/def/voc/texture/> .
@prefix sosa: <http://www.w3.org/ns/sosa/> .
@prefix ssn-ext: <http://www.w3.org/ns/ssn/ext/> .
@prefix struct-corveg: <http://linked.data.gov.au/dataset/corveg/structure/> .
@prefix time: <http://www.w3.org/2006/time#> .
@prefix unit: <http://qudt.org/vocab/unit/> .
@prefix v-comm-corveg: <http://linked.data.gov.au/dataset/corveg/vege-community/> .
@prefix xml: <http://www.w3.org/XML/1998/namespace> .
@prefix xsd: <http://www.w3.org/2001/XMLSchema#> .

cv-corveg:disturbance-type a owl:Ontology ;
    owl:imports <http://www.w3.org/2004/02/skos/core>,
        sosa: .

cv-corveg:disturbance-type-erosion a skos:Concept,
        sosa:Result ;
    skos:definition "Area type and severity of erosion." ;
    skos:hiddenLabel "13" ;
    skos:inScheme cv-corveg:disturbance-types ;
    skos:notation "Erosion" ;
    skos:prefLabel "Erosion" .

cv-corveg:disturbance-type-extensive_clearing a skos:Concept,
        sosa:Result ;
    skos:definition "Most of the vegetation is regrowth from a previous clearing/thinning event." ;
    skos:hiddenLabel "7" ;
    skos:inScheme cv-corveg:disturbance-types ;
    skos:notation "Extensive Clearing" ;
    skos:prefLabel "Extensive Clearing" .

cv-corveg:disturbance-type-feral_digging a skos:Concept,
        sosa:Result ;
    skos:definition "Presence of feral diggings." ;
    skos:hiddenLabel "10" ;
    skos:inScheme cv-corveg:disturbance-types ;
    skos:notation "Feral Digging" ;
    skos:prefLabel "Feral Digging" .

cv-corveg:disturbance-type-fire a skos:Concept,
        sosa:Result ;
    skos:definition "Proportion of the site burnt, age of fire and tallest vegetation impacted." ;
    skos:hiddenLabel "3" ;
    skos:inScheme cv-corveg:disturbance-types ;
    skos:notation "Fire" ;
    skos:prefLabel "Fire" .

cv-corveg:disturbance-type-flood a skos:Concept,
        sosa:Result ;
    skos:definition "Floods." ;
    skos:hiddenLabel "11" ;
    skos:inScheme cv-corveg:disturbance-types ;
    skos:notation "Flood" ;
    skos:prefLabel "Flood" .

cv-corveg:disturbance-type-grazing a skos:Concept,
        sosa:Result ;
    skos:definition "Grazing by domestic stock, feral animals and native animals evident in damage to the ground layer plants and/or presence of animal faeces or tracks." ;
    skos:hiddenLabel "9" ;
    skos:inScheme cv-corveg:disturbance-types ;
    skos:notation "Grazing" ;
    skos:prefLabel "Grazing" .

cv-corveg:disturbance-type-logging a skos:Concept,
        sosa:Result ;
    skos:definition "Number of logging stumps in the site." ;
    skos:hiddenLabel "5" ;
    skos:inScheme cv-corveg:disturbance-types ;
    skos:notation "Logging" ;
    skos:prefLabel "Logging" .

cv-corveg:disturbance-type-non_remnant a skos:Concept,
        sosa:Result ;
    skos:definition "Not remnant vegetation." ;
    skos:hiddenLabel "12" ;
    skos:inScheme cv-corveg:disturbance-types ;
    skos:notation "Non Remnant" ;
    skos:prefLabel "Non Remnant" .

cv-corveg:disturbance-type-ringbarking-thinning a skos:Concept,
        sosa:Result ;
    skos:definition "Number of stems in the site ringbarked, poisoned or thinned." ;
    skos:hiddenLabel "6" ;
    skos:inScheme cv-corveg:disturbance-types ;
    skos:notation "Ringbarking/thinning" ;
    skos:prefLabel "Ringbarking/thinning" .

cv-corveg:disturbance-type-roadworks a skos:Concept,
        sosa:Result ;
    skos:definition "Proportion of the site damaged by tracks and roads and the age of the damage." ;
    skos:hiddenLabel "2" ;
    skos:inScheme cv-corveg:disturbance-types ;
    skos:notation "Roadworks" ;
    skos:prefLabel "Roadworks" .

cv-corveg:disturbance-type-salinity a skos:Concept,
        sosa:Result ;
    skos:definition "Proportion of the site affected by severe anthropogenic salinity." ;
    skos:hiddenLabel "4" ;
    skos:inScheme cv-corveg:disturbance-types ;
    skos:notation "Salinity" ;
    skos:prefLabel "Salinity" .

cv-corveg:disturbance-type-storm a skos:Concept,
        sosa:Result ;
    skos:definition "Proportion of crown cover damaged by storms on the site and the age of the damage." ;
    skos:hiddenLabel "1" ;
    skos:inScheme cv-corveg:disturbance-types ;
    skos:notation "Storm" ;
    skos:prefLabel "Storm Damage" .

cv-corveg:disturbance-type-weeds a skos:Concept,
        sosa:Result ;
    skos:definition "Percentage cover of exotic species." ;
    skos:hiddenLabel "8" ;
    skos:inScheme cv-corveg:disturbance-types ;
    skos:notation "Weeds" ;
    skos:prefLabel "Weeds" .

cv-corveg:disturbance-types a skos:ConceptScheme ;
    skos:hasTopConcept cv-corveg:disturbance-type-erosion,
        cv-corveg:disturbance-type-extensive_clearing,
        cv-corveg:disturbance-type-feral_digging,
        cv-corveg:disturbance-type-fire,
        cv-corveg:disturbance-type-flood,
        cv-corveg:disturbance-type-grazing,
        cv-corveg:disturbance-type-logging,
        cv-corveg:disturbance-type-non_remnant,
        cv-corveg:disturbance-type-ringbarking-thinning,
        cv-corveg:disturbance-type-roadworks,
        cv-corveg:disturbance-type-salinity,
        cv-corveg:disturbance-type-storm,
        cv-corveg:disturbance-type-weeds ;
    skos:prefLabel "Disturbance type concepts" .

