@prefix apc: <http://linked.data.gov.au/dataset/apc/> .
@prefix apni: <http://linked.data.gov.au/dataset/apni/> .
@prefix biod: <http://linked.data.gov.au/def/biodiversity/> .
@prefix corveg: <http://linked.data.gov.au/dataset/corveg/> .
@prefix corveg-def: <http://linked.data.gov.au/def/corveg/> .
@prefix cv-corveg: <http://linked.data.gov.au/def/corveg-cv/> .
@prefix data: <http://linked.data.gov.au/def/tern-plot-data/> .
@prefix dct: <http://purl.org/dc/terms/> .
@prefix dist-corveg: <http://linked.data.gov.au/dataset/corveg/disturbance/> .
@prefix dwct: <http://rs.tdwg.org/dwc/terms/> .
@prefix epsg-crs: <http://www.opengis.net/def/crs/epsg/0/> .
@prefix geo: <http://www.w3.org/2003/01/geo/wgs84_pos#> .
@prefix geol-corveg: <http://linked.data.gov.au/dataset/corveg/geology/> .
@prefix location-corveg: <http://linked.data.gov.au/dataset/corveg/location/> .
@prefix locn: <http://www.w3.org/ns/locn#> .
@prefix ogroup-corveg: <http://linked.data.gov.au/def/corveg-ogroup/> .
@prefix op-corveg: <http://linked.data.gov.au/def/corveg-op/> .
@prefix owl: <http://www.w3.org/2002/07/owl#> .
@prefix plot: <http://linked.data.gov.au/def/tern-plot/> .
@prefix prov: <http://www.w3.org/ns/prov#> .
@prefix rdf: <http://www.w3.org/1999/02/22-rdf-syntax-ns#> .
@prefix rdfs: <http://www.w3.org/2000/01/rdf-schema#> .
@prefix rfstruct-corveg: <http://linked.data.gov.au/dataset/corveg/rf-structure/> .
@prefix site-corveg: <http://linked.data.gov.au/dataset/corveg/site/> .
@prefix site-strata-corveg: <http://linked.data.gov.au/dataset/corveg/site-strata/> .
@prefix site-tax-strata-corveg: <http://linked.data.gov.au/dataset/corveg/site-tax-strata/> .
@prefix situation-corveg: <http://linked.data.gov.au/dataset/corveg/situation/> .
@prefix skos: <http://www.w3.org/2004/02/skos/core#> .
@prefix soil-corveg: <http://linked.data.gov.au/dataset/corveg/soil/> .
@prefix soil-text-corveg: <http://registry.it.csiro.au/sandbox/soil-data-ie/def/voc/texture/> .
@prefix sosa: <http://www.w3.org/ns/sosa/> .
@prefix ssn-ext: <http://www.w3.org/ns/ssn/ext/> .
@prefix struct-corveg: <http://linked.data.gov.au/dataset/corveg/structure/> .
@prefix time: <http://www.w3.org/2006/time#> .
@prefix unit: <http://qudt.org/vocab/unit/> .
@prefix v-comm-corveg: <http://linked.data.gov.au/dataset/corveg/vege-community/> .
@prefix xml: <http://www.w3.org/XML/1998/namespace> .
@prefix xsd: <http://www.w3.org/2001/XMLSchema#> .

cv-corveg:rainforest-deciduousness a owl:Ontology ;
    owl:imports <http://www.w3.org/2004/02/skos/core>,
        sosa: .

cv-corveg:rainforest-deciduousness-a a skos:Concept,
        sosa:Result ;
    skos:definition "canopy leaves are shed throughout the year, so that there is no discernible loss of canopy at any time." ;
    skos:hiddenLabel "1" ;
    skos:inScheme cv-corveg:rainforest-deciduousnesses ;
    skos:notation "A" ;
    skos:prefLabel "evergreen" .

cv-corveg:rainforest-deciduousness-c a skos:Concept,
        sosa:Result ;
    skos:definition "few or none of the species are obligately deciduous, and most of those that shed their leaves do so incompletely depending on the severity of the dry season." ;
    skos:hiddenLabel "2" ;
    skos:inScheme cv-corveg:rainforest-deciduousnesses ;
    skos:notation "C" ;
    skos:prefLabel "semi-evergreen" .

cv-corveg:rainforest-deciduousness-d a skos:Concept,
        sosa:Result ;
    skos:definition "for all species that shed their leaves, leaf shed is complete, and this behaviour is obligatory and fixed for the species." ;
    skos:hiddenLabel "3" ;
    skos:inScheme cv-corveg:rainforest-deciduousnesses ;
    skos:notation "D" ;
    skos:prefLabel "deciduous" .

cv-corveg:rainforest-deciduousness-e a skos:Concept,
        sosa:Result ;
    skos:definition "some species that lose their leaves are obligately deciduous, and some are facultatively deciduous i.e. leaf-fall is controlled by the severity of the dry season." ;
    skos:hiddenLabel "4" ;
    skos:inScheme cv-corveg:rainforest-deciduousnesses ;
    skos:notation "E" ;
    skos:prefLabel "semi-deciduous" .

cv-corveg:rainforest-deciduousness-unrecorded a skos:Concept,
        sosa:Result ;
    skos:definition "Unrecorded." ;
    skos:hiddenLabel "999" ;
    skos:inScheme cv-corveg:rainforest-deciduousnesses ;
    skos:notation "null" ;
    skos:prefLabel "Unrecorded" .

cv-corveg:rainforest-deciduousnesses a skos:ConceptScheme ;
    skos:hasTopConcept cv-corveg:rainforest-deciduousness-a,
        cv-corveg:rainforest-deciduousness-c,
        cv-corveg:rainforest-deciduousness-d,
        cv-corveg:rainforest-deciduousness-e,
        cv-corveg:rainforest-deciduousness-unrecorded ;
    skos:prefLabel "Rainforest deciduousness concepts" .

